ReadMe.md
@@ -9,3 +9,7 @@ synthesize kbo minimal term r, add rule l -> r
 Alg 1:
 Simplify with R n, if smaller size, discard
 otherwise: smt
+
+
+Alg 2:
+Enumerate terms only from the irreducable set of previous iterations.
